

$$\begin{aligned}\text{perplexity}(W) &= P(w_1 w_2 \dots w_N)^{-\frac{1}{N}} \\ &= \sqrt[N]{\frac{1}{P(w_1 w_2 \dots w_N)}}\end{aligned}\tag{3.14}$$

Or we can use the chain rule to expand the probability of W :

$$\text{perplexity}(W) = \sqrt[N]{\prod_{i=1}^N \frac{1}{P(w_i | w_1 \dots w_{i-1})}}\tag{3.15}$$

$$\text{perplexity}(W) = \sqrt[N]{\frac{1}{P(w_1 w_2 \dots w_N)}}$$

由概率的链式法则得

$$P(w_1 w_2 \dots w_N) = P(w_2 | w_1) \cdot P(w_3 | w_1 w_2) \dots P(w_i | w_1 \dots w_{i-1})$$

$$\text{即 } P(w_1 w_2 \dots w_N) = \prod_{i=1}^N P(w_i | w_1 \dots w_{i-1})$$

代入 perplexity(W)得

$$\text{perplexity}(W) = \sqrt[N]{\prod_{i=1}^N \frac{1}{P(w_i | w_1 \dots w_{i-1})}}$$

得证。